wp pweq wip

theories/diffpriv/coupling_rules_pw_simple.v
@@ -106,6 +106,59 @@ Section rules.
   Qed.
 
 
+  Definition WP_PWEQ_no_K := ∀ e e' E,
+    (
+      ∀ (RES : val),
+      ⤇ e' -∗
+          WP e @ E
+            {{ v, ∃ v' : val, ⤇ (Val v') ∗ ⌜v = RES → v' = RES⌝ }} )
+-∗
+    (⤇ e'
+    -∗
+     WP e @ E
+      {{ v, ∃ v' : val, ⤇ (Val v') ∗ ⌜v = v'⌝ }}).
+
+  Lemma wp_pweq_no_K : (* ∀ (e e' : expr) (* ε δ *),
+       (* state_interp σ ∗ spec_interp (e', σ') ∗ err_interp ε δ ∗ *)
+       (∀ (RES : val), WP e {{ v, ∃ v', ⤇ Val v' ∗ ⌜v = RES → v' = RES⌝ }}) -∗
+       (* state_interp σ ∗ spec_interp (e', σ') ∗ err_interp ε δ ∗ *)
+       ⤇ e' -∗
+       WP e {{ v, ∃ v', ⤇ Val v' ∗ ⌜v = v'⌝ }} *)
+  WP_PWEQ_no_K.
+  Proof.
+    iIntros (???) "pw rhs".
+    rewrite wp_unfold /wp_pre //=.
+    destruct (to_val e) eqn:He.
+    { iSpecialize ("pw" $! v).
+      rewrite wp_unfold /wp_pre //= He. iMod ("pw" with "rhs") as "pw". iModIntro. iDestruct "pw" as "(%v' & v' & %pweq)".
+      iExists v'. iFrame. rewrite pweq => //.
+    }
+    (* iIntros (e1 e1' σ1 σ1' ε δ) "(HT & S & E & pw)". *)
+    iIntros (?????) "(HT & S & ε & δ)".
+    iDestruct (spec_auth_prog_agree with "S rhs") as %->.
+    iApply fupd_mask_intro; [set_solver|]; iIntros "Hclose'".
+    iSplit.
+    { iSpecialize ("pw" $! #42 with "rhs").
+      rewrite wp_unfold /wp_pre //= He. iSpecialize ("pw" with "[$]").
+      admit.
+    }
+    iRight.
+    iNext.
+    iMod "Hclose'".
+    iModIntro. iSplit.
+    - iModIntro. iIntros. iSplit.
+      + iIntros "(%v' & rhs & %eq)". iExists v', σ1'. iSplit. 2: by rewrite eq. admit.
+      + iIntros "(%v' & %σ' & rhs & %eq)". iExists v'. iSplit. 2: by rewrite eq. admit.
+    - iIntros (RES).
+      iApply (wp_strong_mono with "[pw rhs]") => //.
+      + iApply ("pw" $! RES). done.
+      + simpl. iIntros "%v (%v' & rhs & %pweq) !>".
+        iExists v',σ1'.
+        iDestruct (spec_auth_prog_agree with "S rhs") as %->.
+        iSplit. 2: iPureIntro ; exact pweq.
+        iFrame.
+  Admitted.
+
   Definition WP_PWEQ := ∀ e e' K E,
     (
       ∀ (RES : val),
@@ -135,39 +188,24 @@ Section rules.
     }
     (* iIntros (e1 e1' σ1 σ1' ε δ) "(HT & S & E & pw)". *)
     iIntros (?????) "(HT & S & ε & δ)".
+    iDestruct (spec_auth_prog_agree with "S rhs") as %->.
+    iApply fupd_mask_intro; [set_solver|]; iIntros "Hclose'".
+    iSplit. 1: admit.
     iRight.
-
-
-    (* iRevert "pw". (e e' σ σ' ε δ). iLöb as "IH". iIntros (e e' σ σ' ε δ) "pw". *)
-    destruct (to_val e1) eqn:ev.
-    - rewrite wp_unfold /wp_pre //=.
-      iSpecialize ("pw" $! v).
-      (* iSpecialize ("pw" with "[$rhs]"). *)
-      rewrite wp_unfold /wp_pre /=. rewrite ev /=.
-      iMod "pw" as "(%v' & rhs & %pweq)".
-      iModIntro. iExists v'. iFrame. rewrite pweq => //.
-    -
-      rewrite wp_unfold /wp_pre //=.
-      (* clear ε δ e1' σ1 σ1'. *)
-      iIntros (?????). iIntros "((H & T) & S & ε & δ)".
-
-      iSpecialize ("pw" $! #42).
-
-      setoid_rewrite wp_unfold at 3. rewrite /wp_pre //= ev /=.
-      iSpecialize ("pw" with "[$H $T $S $ε $δ]").
-      iMod "pw" as "(%red & %Rpw & % & % & % & % & %CPL & %hε & %hδ & pw)".
-      iModIntro ; iSplit ; [done|].
-      iExists Rpw, ε1, ε2, δ1, δ2. repeat iSplit ; [done|done|done|].
-      iIntros (???? HR).
-      iSpecialize ("pw" $! _ _ _ _ HR).
-      iNext.
-      iMod "pw" as "(HT & S & E & Hrec)". iModIntro. iFrame.
-      iSpecialize ("IH" $! e2 e2' σ2 σ2').
-      iApply "IH".
-      iIntros.
-      assert (RES = #42) as -> by admit.
-      iApply "Hrec".
-
+    iNext.
+    iMod "Hclose'".
+    iModIntro. iSplit.
+    - iModIntro. iIntros. iSplit.
+      + iIntros "(%v' & rhs & %eq)". iExists v', σ1'. iSplit. 2: by rewrite eq. admit.
+      + iIntros "(%v' & %σ' & rhs & %eq)". iExists v'. iSplit. 2: by rewrite eq. admit.
+    - iIntros (RES).
+      iApply (wp_strong_mono with "[pw rhs]") => //.
+      + iApply ("pw" $! RES). done.
+      + simpl. iIntros "%v (%v' & rhs & %pweq) !>".
+        iExists v',σ1'.
+        iDestruct (spec_auth_prog_agree with "S rhs") as %->.
+        iSplit. 2: iPureIntro ; exact pweq.
+        iFrame.
   Admitted.
 
   (* Lemma wp_couple_laplace (loc loc' k k' : Z)
